EthCryptographySpecs/Proofs/Kzg.lean
@@ -2,6 +2,7 @@ import EthCryptographySpecs.Proofs.Kzg.BitReversal
 import EthCryptographySpecs.Proofs.Kzg.Fft
 import EthCryptographySpecs.Proofs.Kzg.Polynomials
 import EthCryptographySpecs.Proofs.Kzg.Core
+import EthCryptographySpecs.Proofs.Kzg.Recovery
 
 /-!
 # `EthCryptographySpecs.Proofs.Kzg`
